src/goose_lang/lib/slice/slice.v
@@ -1,8 +1,8 @@
 From RecordUpdate Require Import RecordSet.
 From Perennial.Helpers Require Import List Fractional.
 From Perennial.goose_lang Require Import proofmode array.
-From Perennial.goose_lang.lib Require Import persistent_readonly.
-From Perennial.goose_lang.lib Require Export slice.impl typed_mem.
+From Perennial.goose_lang.lib Require Import persistent_readonly typed_mem.
+From Perennial.goose_lang.lib Require Export slice.impl.
 From Perennial.goose_lang.lib Require Import control.control.
 
 Set Default Proof Using "Type".
