src/program_proof/disk_prelude.v
@@ -1,4 +1,7 @@
 From Perennial.program_proof Require Export proof_prelude.
+(* For backwards compat, make untyped slice lib take precedence. *)
+From Perennial.goose_lang.lib Require Export slice.
+
 From Perennial.goose_lang Require Export ffi.disk_prelude.
 
 (* Make sure Z_scope is open. *)
