src/program_proof/memkv/memkv_get_proof.v
@@ -307,7 +307,7 @@ Proof.
       iDestruct "HownShard" as "[%Hbad|HownShard]".
       { exfalso. done. }
       iDestruct "HownShard" as (kvs_ptr m mv) "(HshardGhost & %Hkvs_lookup & %Hkvs_dom & HkvsMap & HvalSlices)".
-      wp_apply (wp_SliceGet _ _ _ _ _ _ _ (#kvs_ptr) with "[Hkvss_sl]").
+      wp_apply (slice.wp_SliceGet _ _ _ _ _ _ _ (#kvs_ptr) with "[Hkvss_sl]").
       {
         iFrame "Hkvss_sl".
         iPureIntro.
