src/program_proof/std_proof.v
@@ -32,18 +32,18 @@ Proof.
 Qed.
 
 Lemma wp_BytesEqual (x y : Slice.t) (xs ys : list byte) qx qy :
-  {{{ typed_slice.is_slice_small x byteT qx xs ∗
-      typed_slice.is_slice_small y byteT qy ys }}}
+  {{{ is_slice_small x byteT qx xs ∗
+      is_slice_small y byteT qy ys }}}
     BytesEqual (slice_val x) (slice_val y)
   {{{ RET #(bool_decide (xs = ys));
-      typed_slice.is_slice_small x byteT qx xs ∗
-      typed_slice.is_slice_small y byteT qy ys }}}.
+      is_slice_small x byteT qx xs ∗
+      is_slice_small y byteT qy ys }}}.
 Proof.
   iIntros (Φ) "[Hx Hy] HΦ". wp_lam. wp_pures.
   do 2 wp_apply wp_slice_len.
   wp_pures.
-  iDestruct (typed_slice.is_slice_small_sz with "Hx") as %Hxlen.
-  iDestruct (typed_slice.is_slice_small_sz with "Hy") as %Hylen.
+  iDestruct (is_slice_small_sz with "Hx") as %Hxlen.
+  iDestruct (is_slice_small_sz with "Hy") as %Hylen.
   assert (#x.(Slice.sz) = #(length xs))%V as ->.
   { rewrite Hxlen. do 2 f_equal. word. }
   assert (#y.(Slice.sz) = #(length ys))%V as ->.
@@ -100,11 +100,11 @@ Proof.
   destruct (lookup_lt_is_Some_2 ys i) as [yi Hyi]; first by rewrite -Hlens.
   wp_load.
   (* FIXME: some typeclass is set up wrong so TC inference picks the wrong type here *)
-  wp_apply (typed_slice.wp_SliceGet (V:=u8) with "[$Hx]").
+  wp_apply (wp_SliceGet (V:=u8) with "[$Hx]").
   { replace (int.nat i) with i by word. done. }
   iIntros "Hx".
   wp_load.
-  wp_apply (typed_slice.wp_SliceGet (V:=u8) with "[$Hy]").
+  wp_apply (wp_SliceGet (V:=u8) with "[$Hy]").
   { replace (int.nat i) with i by word. done. }
   iIntros "Hy".
   wp_pures.
